Almost finished the Splay Heap.
In general these proofs look far grungier than Arthur's Coq proofs (which I
admittedly can't read very well).  This may be partially be because of my
stylistic choice to split the heap invariant into 2 functions, instead of 1
relation.  However, the HOL proofs are full of BAG grunge, whereas Coq seem to
be doing alot more of the multiset reasoning for him.

examples/miniML/okasaki-examples/SplayHeapScript.sml
@@ -1,5 +1,5 @@
 open bossLib Theory Parse boolTheory pairTheory Defn Tactic boolLib bagTheory
-open relationTheory lcsymtacs;
+open relationTheory bagLib lcsymtacs;
 
 val fs = full_simp_tac (srw_ss ())
 val rw = srw_tac []
@@ -11,6 +11,36 @@ val full_case_tac = BasicProvers.FULL_CASE_TAC;
 
 
 val _ = new_theory "SplayHeap"
+
+val WeakLinearOrder_neg = Q.prove (
+`!leq x y. WeakLinearOrder leq ⇒ (~leq x y = leq y x ∧ x ≠ y)`,
+metis_tac [WeakLinearOrder, WeakOrder, trichotomous, reflexive_def,
+           antisymmetric_def]);
+
+val BAG_EVERY_DIFF = Q.prove (
+`!P b1 b2. BAG_EVERY P b1 ⇒ BAG_EVERY P (BAG_DIFF b1 b2)`,
+rw [BAG_EVERY] >>
+metis_tac [BAG_IN_DIFF_E]);
+
+val BAG_EVERY_EL = Q.prove (
+`!P x. BAG_EVERY P (EL_BAG x) = P x`,
+rw [BAG_EVERY, EL_BAG]);
+
+val BAG_INN_BAG_DIFF = Q.prove (
+`!x m b1 b2. 
+  BAG_INN x m (BAG_DIFF b1 b2) = 
+  ∃n1 n2. (m = n1 - n2) ∧ 
+          BAG_INN x n1 b1 ∧ BAG_INN x n2 b2 ∧ ~BAG_INN x (n2 + 1) b2`,
+rw [BAG_INN, BAG_DIFF] >>
+EQ_TAC >>
+rw [] >|
+[qexists_tac `b2 x + m` >>
+     qexists_tac `b2 x` >>
+     decide_tac,
+ qexists_tac `0` >>
+     qexists_tac `b2 x` >>
+     decide_tac,
+ decide_tac]);
 
 val _ = Hol_datatype `
 heaps = Empty | Node of heaps => 'a => heaps`;
@@ -26,7 +56,7 @@ val splay_heap_ok_def = Define `
   splay_heap_ok leq h1 ∧
   splay_heap_ok leq h2 ∧
   BAG_EVERY (\y. leq y x) (splay_heap_to_bag h1) ∧
-  BAG_EVERY (\y. ¬leq y x) (splay_heap_to_bag h2))`;
+  BAG_EVERY (\y. leq x y) (splay_heap_to_bag h2))`;
 
 val _ = Define `
 empty = Empty`;
@@ -118,32 +148,49 @@ rw [] >>
 fs [BAG_EVERY, transitive_def, trichotomous] >>
 metis_tac []);
 
-(*
+val partition_ok_lem = Q.prove (
+`!leq p h1 h2 h3.
+  (partition leq p h1 = (h2, h3)) ⇒ 
+  BAG_EVERY P (splay_heap_to_bag h1) ⇒
+  BAG_EVERY P (splay_heap_to_bag h2) ∧
+  BAG_EVERY P (splay_heap_to_bag h3)`,
+rw [] >>
+`splay_heap_to_bag h1 = 
+ BAG_UNION (splay_heap_to_bag h2) (splay_heap_to_bag h3)`
+          by metis_tac [partition_bags] >>
+rw [] >>
+fs [] >>
+rw []);
+
 val partition_ok = Q.prove (
 `!leq p h1 h2 h3.
-  transitive leq ∧ 
-  trichotomous leq ∧
+  WeakLinearOrder leq ∧
   ((h2,h3) = partition leq p h1) ∧
   splay_heap_ok leq h1
   ⇒
   splay_heap_ok leq h2 ∧
   splay_heap_ok leq h3`,
 recInduct partition_ind >>
-rw [partition_def, splay_heap_ok_def] >>
-
+RW_TAC pure_ss [] >> 
+cases_on `leq x pivot` >>
+fs [partition_def, splay_heap_ok_def] >>
 every_case_tac >>
 fs [] >>
 rw [] >>
 cases_on `partition leq pivot h0` >>
 cases_on `partition leq pivot h` >>
-fs [LET_THM, splay_heap_ok_def] >>
-metis_tac [partition_split]
-rw []
-
-, splay_heap_ok_def, splay_heap_to_bag_def] >>
-rw [splay_heap_ok_def]
-metis_tac [ASSOC_BAG_UNION, COMM_BAG_UNION, BAG_INSERT_commutes]);
-*)
+fs [LET_THM, splay_heap_ok_def, splay_heap_to_bag_def] >>
+rw [] >-
+(fs [BAG_EVERY] >>
+ metis_tac [transitive_def, WeakLinearOrder, WeakOrder]) >-
+metis_tac [partition_ok_lem] >-
+metis_tac [partition_ok_lem] >-
+metis_tac [partition_ok_lem] >-
+metis_tac [partition_ok_lem] >-
+metis_tac [partition_ok_lem] >-
+metis_tac [partition_ok_lem] >-
+(fs [BAG_EVERY] >>
+ metis_tac [transitive_def, WeakLinearOrder, WeakOrder]));
 
 val insert_def = Define `
 insert leq x t =
@@ -159,10 +206,10 @@ val merge_def = tDefine "merge" `
                         heaps_size (\_.1) y +
                         heaps_size (\_.1) z)` >>
  rw [] >>
- imp_res_tac partition_thm >>
+ imp_res_tac partition_size >>
  pop_assum (MP_TAC o Q.SPEC `(λ_.1)`) >>
  pop_assum (MP_TAC o Q.SPEC `(λ_.1)`) >>
- full_simp_tac (srw_ss() ++ ARITH_ss) [partition_thm]);
+ full_simp_tac (srw_ss() ++ ARITH_ss) [partition_size]);
 
 val merge_ind = fetch "-" "merge_ind"
 
@@ -172,12 +219,14 @@ val find_min_def = Define `
 
 val find_min_ind = fetch "-" "find_min_ind"
 
-val delete_min_defn = Define `
+val delete_min_def = Define `
 (delete_min (Node Empty x b) = b) ∧
 (delete_min (Node (Node Empty x b) y c) = Node b y c) ∧
 (delete_min (Node (Node a x b) y c) = Node (delete_min a) x (Node b y c))`;
 
-val insert_thm = Q.store_thm ("insert_thm",
+val delete_min_ind = fetch "-" "delete_min_ind"
+
+val splay_heap_insert_bag = Q.store_thm ("splay_heap_insert_bag",
 `!h leq x.
   splay_heap_to_bag (insert leq x h) =
   BAG_INSERT x (splay_heap_to_bag h)`,
@@ -185,16 +234,25 @@ induct_on `h` >>
 rw [splay_heap_to_bag_def, insert_def] >>
 rw [splay_heap_to_bag_def] >>
 fs [insert_def] >>
-imp_res_tac (GSYM partition_thm) >>
+imp_res_tac (GSYM partition_bags) >>
 fs [splay_heap_to_bag_def]);
 
-val insert_ok = Q.store_thm ("insert_ok",
-`!leq x h. splay_heap_ok leq h ⇒ splay_heap_ok leq (insert leq x h)`,
-induct_on `h` >>
-rw [splay_heap_ok_def, insert_def] >>
-rw [splay_heap_ok_def] >>
+val splay_heap_insert_ok = Q.store_thm ("splay_heap_insert_ok",
+`!leq x h. 
+  WeakLinearOrder leq ∧ splay_heap_ok leq h 
+  ⇒ 
+  splay_heap_ok leq (insert leq x h)`,
+rw [insert_def, splay_heap_ok_def] >>
+rw [splay_heap_ok_def] >-
+metis_tac [partition_ok] >-
+metis_tac [partition_ok] >-
+metis_tac [WeakLinearOrder, WeakOrder, partition_split] >-
+(`BAG_EVERY (\y. ¬leq y x) (splay_heap_to_bag b)` 
+           by metis_tac [partition_split, WeakLinearOrder, WeakOrder] >>
+ fs [BAG_EVERY] >>
+ metis_tac [WeakLinearOrder_neg]));
 
-val merge_thm = Q.store_thm ("merge_thm",
+val splay_heap_merge_bag = Q.store_thm ("splay_heap_merge_bag",
 `!leq h1 h2.
   (splay_heap_to_bag (merge leq h1 h2) =
     BAG_UNION (splay_heap_to_bag h1) (splay_heap_to_bag h2))`,
@@ -202,19 +260,88 @@ recInduct merge_ind >>
 rw [merge_def, splay_heap_to_bag_def] >>
 cases_on `partition leq x h2` >>
 fs [] >>
-imp_res_tac (GSYM partition_thm) >>
+imp_res_tac (GSYM partition_bags) >>
 rw [splay_heap_to_bag_def, BAG_UNION_INSERT] >>
 metis_tac [ASSOC_BAG_UNION, COMM_BAG_UNION, BAG_INSERT_commutes]);
 
-(*
-val find_min_thm = Q.prove (
-`!h x leq. (h ≠ Empty) ∧ splay_heap_ok leq h ⇒
+val splay_heap_merge_ok = Q.store_thm ("splay_heap_merge_ok",
+`!leq h1 h2.
+  WeakLinearOrder leq ∧ splay_heap_ok leq h1 ∧ splay_heap_ok leq h2 
+  ⇒ 
+  splay_heap_ok leq (merge leq h1 h2)`,
+recInduct merge_ind >>
+rw [merge_def, splay_heap_ok_def] >>
+rw [splay_heap_ok_def, splay_heap_merge_bag] >-
+metis_tac [partition_ok] >-
+metis_tac [partition_ok] >-
+metis_tac [partition_split, WeakLinearOrder, WeakOrder] >-
+(`BAG_EVERY (\y. ¬leq y x) (splay_heap_to_bag tb)` 
+           by metis_tac [partition_split, WeakLinearOrder, WeakOrder] >>
+ fs [BAG_EVERY] >>
+ metis_tac [WeakLinearOrder_neg]));
+
+val splay_heap_find_min = Q.prove (
+`!h x leq. WeakLinearOrder leq ∧ (h ≠ Empty) ∧ splay_heap_ok leq h ⇒
   ((find_min h = x) =
    (BAG_IN x (splay_heap_to_bag h) ∧
     (!y. BAG_IN y (splay_heap_to_bag h) ⇒ leq x y)))`,
 recInduct find_min_ind >>
 rw [splay_heap_to_bag_def, splay_heap_ok_def, find_min_def] >-
-*)
+metis_tac [BAG_EVERY, WeakLinearOrder_neg, WeakLinearOrder, WeakOrder, 
+           reflexive_def] >>
+EQ_TAC >>
+rw [] >-
+metis_tac [] >-
+(fs [BAG_EVERY] >>
+ metis_tac [WeakLinearOrder, WeakOrder, transitive_def]) >-
+metis_tac [] >-
+metis_tac [] >-
+metis_tac [] >-
+(fs [BAG_EVERY] >>
+ metis_tac [WeakLinearOrder, WeakOrder, transitive_def]) >-
+metis_tac [BAG_EVERY, WeakLinearOrder_neg, WeakLinearOrder, WeakOrder, 
+           reflexive_def] >-
+metis_tac [] >-
+metis_tac [] >-
+metis_tac [] >-
+metis_tac [BAG_EVERY, WeakLinearOrder_neg, WeakLinearOrder, WeakOrder, 
+           reflexive_def]);
+
+val splay_heap_find_min_thm = Q.store_thm ("splay_heap_find_min_thm",
+`!h leq. WeakLinearOrder leq ∧ (h ≠ Empty) ∧ splay_heap_ok leq h ⇒
+  BAG_IN (find_min h) (splay_heap_to_bag h) ∧
+  (!y. BAG_IN y (splay_heap_to_bag h) ⇒ leq (find_min h) y)`,
+metis_tac [splay_heap_find_min]);
+
+val splay_heap_delete_min_thm = Q.store_thm ("splay_heap_delete_min_thm",
+`!h leq. 
+  WeakLinearOrder leq ∧
+  (h ≠ Empty) ∧ 
+  splay_heap_ok leq h 
+  ⇒ 
+  splay_heap_ok leq (delete_min h) ∧
+  (splay_heap_to_bag (delete_min h) = 
+   BAG_DIFF (splay_heap_to_bag h) (EL_BAG (find_min h)))`,
+HO_MATCH_MP_TAC delete_min_ind >>
+srw_tac [bagLib.BAG_ss] 
+        [delete_min_def, splay_heap_ok_def, splay_heap_to_bag_def,
+         find_min_def, BAG_INSERT_UNION] >|
+[res_tac >>
+     rw [] >>
+     match_mp_tac BAG_EVERY_DIFF >>
+     rw [],
+ fs [BAG_EVERY_EL],
+ fs [BAG_EVERY_EL] >>
+     fs [BAG_EVERY] >>
+     metis_tac [WeakLinearOrder, WeakOrder, transitive_def],
+ res_tac >>
+     srw_tac [BAG_AC_ss] [] >>
+     (* EL_BAG (find_min (Node v6 v7 v8)) is a subbag of 
+        EL_BAG v7 ⊎ (splay_heap_to_bag v6 ⊎ splay_heap_to_bag v8)
+        by splay_heap_find_min_thm, and so by BAG_UNION_DIFF the difference
+        can be lifted out to the top.  I don't feel like bashing this through
+        HOL at the moment. *)
+     all_tac]);
 
 val _ = export_theory()
 
